Weidenbach_Book/IsaSAT/IsaSAT_LLVM.thy
@@ -1,5 +1,6 @@
 theory IsaSAT_LLVM
   imports
+    IsaSAT_Print_LLVM
     IsaSAT_CDCL_LLVM
     IsaSAT_Initialisation_LLVM
     IsaSAT_Restart_Simp_LLVM
@@ -9,6 +10,16 @@ begin
 hide_const (open)array_assn
 
 hide_const (open)IICF_Multiset.mset_rel
+hide_const (open) NEMonad.ASSERT NEMonad.RETURN
+
+lemma convert_state_hnr:
+  \<open>(uncurry (Mreturn oo (\<lambda>_ S. S)), uncurry (RETURN oo convert_state))
+   \<in> ghost_assn\<^sup>k *\<^sub>a (isasat_init_assn)\<^sup>d \<rightarrow>\<^sub>a
+     isasat_init_assn\<close>
+  unfolding convert_state_def
+  by sepref_to_hoare vcg
+
+declare convert_state_hnr[sepref_fr_rules]
 
 chapter \<open>Code of Full IsaSAT\<close>
 
@@ -232,7 +243,6 @@ lemma [sepref_fr_rules]: \<open>(Mreturn o (\<lambda>_. ()), RETURN o virtual_co
 proof -
   have [simp]: \<open>(\<lambda>s. (\<exists>xa. (\<up>(xa = x)) s)) = (\<up>True)\<close> for s :: \<open>'b::sep_algebra\<close> and x :: 'a
     by (auto simp: pred_lift_extract_simps)
-
   show ?thesis
     unfolding virtual_copy_def ghost_assn_def virtual_copy_rel_def
     apply sepref_to_hoare
@@ -262,20 +272,6 @@ schematic_goal mk_free_ghost_assn[sepref_frame_free_rules]: \<open>MK_FREE ghost
   unfolding ghost_assn_def
   by synthesize_free
 
-lemma convert_state_hnr:
-  \<open>(uncurry (Mreturn oo (\<lambda>_ S. S)), uncurry (RETURN oo convert_state))
-   \<in> ghost_assn\<^sup>k *\<^sub>a (isasat_init_assn)\<^sup>d \<rightarrow>\<^sub>a
-     isasat_init_assn\<close>
-  unfolding convert_state_def
-  by sepref_to_hoare vcg
-declare convert_state_hnr[sepref_fr_rules]
-
-schematic_goal mk_free_isasat_init_assn[sepref_frame_free_rules]: \<open>MK_FREE isasat_init_assn ?fr\<close>
-  unfolding isasat_init_assn_def
-  apply (rule tuple15_free)
-  by synthesize_free+
-
-
 sepref_def IsaSAT_code
   is \<open>uncurry IsaSAT_bounded_heur\<close>
   :: \<open>opts_assn\<^sup>d *\<^sub>a (clauses_ll_assn)\<^sup>k \<rightarrow>\<^sub>a bool1_assn \<times>\<^sub>a model_stat_assn\<close>
@@ -296,200 +292,11 @@ sepref_def IsaSAT_code
   apply (annot_snat_const \<open>TYPE(64)\<close>)
   by sepref
 
-definition print_propa :: \<open>64 word \<Rightarrow> unit\<close> where
-  \<open>print_propa _ = ()\<close>
-
-definition print_confl :: \<open>64 word \<Rightarrow> unit\<close> where
-  \<open>print_confl _ = ()\<close>
-
-definition print_dec :: \<open>64 word \<Rightarrow> unit\<close> where
-  \<open>print_dec _ = ()\<close>
-
-definition print_res :: \<open>64 word \<Rightarrow> unit\<close> where
-  \<open>print_res _ = ()\<close>
-
-definition print_lres :: \<open>64 word \<Rightarrow> unit\<close> where
-  \<open>print_lres _ = ()\<close>
-
-definition print_uset :: \<open>64 word \<Rightarrow> unit\<close> where
-  \<open>print_uset _ = ()\<close>
-
-definition print_gcs :: \<open>64 word \<Rightarrow> unit\<close> where
-  \<open>print_gcs _ = ()\<close>
-
-definition print_binary_unit :: \<open>64 word \<Rightarrow> unit\<close> where
-  \<open>print_binary_unit _ = ()\<close>
-
-definition print_binary_red_removed :: \<open>64 word \<Rightarrow> unit\<close> where
-  \<open>print_binary_red_removed _ = ()\<close>
-
-definition print_purelit_elim :: \<open>64 word \<Rightarrow> unit\<close> where
-  \<open>print_purelit_elim _ = ()\<close>
-
-definition print_purelit_rounds :: \<open>64 word \<Rightarrow> unit\<close> where
-  \<open>print_purelit_rounds _ = ()\<close>
-
-definition print_lbds :: \<open>64 word \<Rightarrow> unit\<close> where
-  \<open>print_lbds _ = ()\<close>
-
-definition print_forward_rounds :: \<open>64 word \<Rightarrow> unit\<close> where
-  \<open>print_forward_rounds _ = ()\<close>
-
-definition print_forward_subsumed :: \<open>64 word \<Rightarrow> unit\<close> where
-  \<open>print_forward_subsumed _ = ()\<close>
-
-definition print_forward_strengthened :: \<open>64 word \<Rightarrow> unit\<close> where
-  \<open>print_forward_strengthened _ = ()\<close>
-
-sepref_def print_propa_impl
-  is \<open>RETURN o print_propa\<close>
-  :: \<open>word_assn\<^sup>k \<rightarrow>\<^sub>a unit_assn\<close>
-  unfolding print_propa_def
-  by sepref
-
-sepref_def print_confl_impl
-  is \<open>RETURN o print_confl\<close>
-  :: \<open>word_assn\<^sup>k \<rightarrow>\<^sub>a unit_assn\<close>
-  unfolding print_confl_def
-  by sepref
-
-sepref_def print_dec_impl
-  is \<open>RETURN o print_dec\<close>
-  :: \<open>word_assn\<^sup>k \<rightarrow>\<^sub>a unit_assn\<close>
-  unfolding print_dec_def
-  by sepref
-
-sepref_def print_res_impl
-  is \<open>RETURN o print_res\<close>
-  :: \<open>word_assn\<^sup>k \<rightarrow>\<^sub>a unit_assn\<close>
-  unfolding print_res_def
-  by sepref
-
-sepref_def print_lres_impl
-  is \<open>RETURN o print_lres\<close>
-  :: \<open>word_assn\<^sup>k \<rightarrow>\<^sub>a unit_assn\<close>
-  unfolding print_lres_def
-  by sepref
-
-sepref_def print_uset_impl
-  is \<open>RETURN o print_uset\<close>
-  :: \<open>word_assn\<^sup>k \<rightarrow>\<^sub>a unit_assn\<close>
-  unfolding print_uset_def
-  by sepref
-
-definition print_irred_clss :: \<open>64 word \<Rightarrow> unit\<close> where
-  \<open>print_irred_clss _ = ()\<close>
-
-sepref_def print_gc_impl
-  is \<open>RETURN o print_gcs\<close>
-  :: \<open>word_assn\<^sup>k \<rightarrow>\<^sub>a unit_assn\<close>
-  unfolding print_gcs_def
-  by sepref
-
-sepref_def print_irred_clss_impl
-  is \<open>RETURN o print_irred_clss\<close>
-  :: \<open>word_assn\<^sup>k \<rightarrow>\<^sub>a unit_assn\<close>
-  unfolding print_irred_clss_def
-  by sepref
-
-sepref_def print_binary_unit_impl
-  is \<open>RETURN o print_binary_unit\<close>
-  :: \<open>word_assn\<^sup>k \<rightarrow>\<^sub>a unit_assn\<close>
-  unfolding print_binary_unit_def
-  by sepref
-
-sepref_def print_purelit_rounds_impl
-  is \<open>RETURN o print_purelit_rounds\<close>
-  :: \<open>word_assn\<^sup>k \<rightarrow>\<^sub>a unit_assn\<close>
-  unfolding print_purelit_rounds_def
-  by sepref
-
-sepref_def print_purelit_elim_impl
-  is \<open>RETURN o print_purelit_elim\<close>
-  :: \<open>word_assn\<^sup>k \<rightarrow>\<^sub>a unit_assn\<close>
-  unfolding print_purelit_elim_def
-  by sepref
-
-sepref_def print_binary_red_removed_impl
-  is \<open>RETURN o print_binary_red_removed\<close>
-  :: \<open>word_assn\<^sup>k \<rightarrow>\<^sub>a unit_assn\<close>
-  unfolding print_binary_red_removed_def
-  by sepref
-
-sepref_def print_forward_rounds_impl
-  is \<open>RETURN o print_forward_rounds\<close>
-  :: \<open>word_assn\<^sup>k \<rightarrow>\<^sub>a unit_assn\<close>
-  unfolding print_forward_rounds_def
-  by sepref
-
-sepref_def print_forward_subsumed_impl
-  is \<open>RETURN o print_forward_subsumed\<close>
-  :: \<open>word_assn\<^sup>k \<rightarrow>\<^sub>a unit_assn\<close>
-  unfolding print_forward_subsumed_def
-  by sepref
-
-sepref_def print_forward_strengthened_impl
-  is \<open>RETURN o print_forward_strengthened\<close>
-  :: \<open>word_assn\<^sup>k \<rightarrow>\<^sub>a unit_assn\<close>
-  unfolding print_forward_strengthened_def
-  by sepref
-
-
-(*TODO Move*)
-definition Subsumption_Stats_rounds where
-  \<open>Subsumption_Stats_rounds = (\<lambda>(rounds, strengthened, subsumed, _). rounds)\<close>
-definition Subsumption_Stats_subsumed where
-  \<open>Subsumption_Stats_subsumed = (\<lambda>(subsumed, strengthened, subsumed, _). subsumed)\<close>
-definition Subsumption_Stats_strengthened where
-  \<open>Subsumption_Stats_strengthened = (\<lambda>(rounds, strengethened, subsumed, _). strengethened)\<close>
-
-definition stats_forward_rounds :: \<open>isasat_stats \<Rightarrow> _\<close> where
-  \<open>stats_forward_rounds = Subsumption_Stats_rounds o get_subsumption_stats\<close>
-
-definition stats_forward_subsumed :: \<open>isasat_stats \<Rightarrow> _\<close> where
-  \<open>stats_forward_subsumed = Subsumption_Stats_subsumed o get_subsumption_stats\<close>
-
-definition stats_forward_strengthened :: \<open>isasat_stats \<Rightarrow> _\<close> where
-  \<open>stats_forward_strengthened = Subsumption_Stats_strengthened o get_subsumption_stats\<close>
-
-sepref_def Subsumption_Stats_rounds_impl
-  is \<open>RETURN o Subsumption_Stats_rounds\<close>
-  :: \<open>subsumption_stats_assn\<^sup>d \<rightarrow>\<^sub>a word64_assn\<close>
-  unfolding subsumption_stats_assn_def Subsumption_Stats_rounds_def
-  by sepref
-sepref_def Subsumption_Stats_strengthened_impl
-  is \<open>RETURN o Subsumption_Stats_strengthened\<close>
-  :: \<open>subsumption_stats_assn\<^sup>d \<rightarrow>\<^sub>a word64_assn\<close>
-  unfolding subsumption_stats_assn_def Subsumption_Stats_strengthened_def
-  by sepref
-sepref_def Subsumption_Stats_subsumed_impl
-  is \<open>RETURN o Subsumption_Stats_subsumed\<close>
-  :: \<open>subsumption_stats_assn\<^sup>d \<rightarrow>\<^sub>a word64_assn\<close>
-  unfolding subsumption_stats_assn_def Subsumption_Stats_subsumed_def
-  by sepref
-sepref_def stats_forward_rounds_impl
-  is \<open>RETURN o stats_forward_rounds\<close>
-  :: \<open>isasat_stats_assn\<^sup>d \<rightarrow>\<^sub>a word64_assn\<close>
-  unfolding stats_forward_rounds_def stats_code_unfold
-  by sepref
-sepref_def stats_forward_subsumed_impl
-  is \<open>RETURN o stats_forward_subsumed\<close>
-  :: \<open>isasat_stats_assn\<^sup>d \<rightarrow>\<^sub>a word64_assn\<close>
-  unfolding stats_forward_subsumed_def stats_code_unfold
-  by sepref
-
-sepref_def stats_forward_strengthened_impl
-  is \<open>RETURN o stats_forward_strengthened\<close>
-  :: \<open>isasat_stats_assn\<^sup>d \<rightarrow>\<^sub>a word64_assn\<close>
-  unfolding stats_forward_strengthened_def stats_code_unfold
-  by sepref
-(*End Move*)
 
 sepref_register print_forward_rounds print_forward_subsumed print_forward_strengthened
 
 abbreviation (input) C_bool_to_bool :: \<open>8 word \<Rightarrow> bool\<close> where
   \<open>C_bool_to_bool g \<equiv> g \<noteq> 0\<close>
-
 
 definition IsaSAT_bounded_heur_wrapper :: \<open>8 word \<Rightarrow> 8 word \<Rightarrow> 8 word \<Rightarrow> 64 word \<Rightarrow> 64 word \<Rightarrow> nat \<Rightarrow>
   8 word \<Rightarrow> 64 word \<Rightarrow> 64 word \<Rightarrow> 64 word \<Rightarrow> _ \<Rightarrow> (nat) nres\<close>where
@@ -512,8 +319,9 @@ definition IsaSAT_bounded_heur_wrapper :: \<open>8 word \<Rightarrow> 8 word \<R
       let _ = print_purelit_elim (stats_pure_lits_removed stats);
       let _ = print_purelit_rounds (stats_pure_lits_rounds stats);
       let _ = print_forward_rounds (stats_forward_rounds stats);
-      let _ = print_forward_subsumed (stats_forward_subsumed stats);
-      let _ = print_forward_strengthened (stats_forward_strengthened stats);
+      let _ = print_forward_tried (stats_forward_tried stats);
+      let _ = print_forward_subsumed (stats_forward_subsumed stats) (stats_forward_tried stats);
+      let _ = print_forward_strengthened (stats_forward_strengthened stats) (stats_forward_tried stats);
       RETURN ((if b then 2 else 0) + (if b' then 1 else 0))
   }\<close>
 
@@ -558,7 +366,7 @@ sepref_definition llvm_version
   is \<open>uncurry0 (RETURN (
         let str = map (nat_of_integer o (of_char :: _ \<Rightarrow> integer)) (String.explode Version.version) @ [0] in
         array_of_version 0 str (replicate (length str) 0)))\<close>
-  :: \<open>unit_assn\<^sup>k \<rightarrow>\<^sub>a array_assn sint32_nat_assn\<close>
+  :: \<open>unit_assn\<^sup>k \<rightarrow>\<^sub>a IICF_Array.array_assn sint32_nat_assn\<close>
   supply[[goals_limit=1]]
   unfolding Version.version_def String.explode_code
     String.asciis_of_Literal
