Weidenbach_Book/IsaSAT/IsaSAT_Print_LLVM.thy
@@ -1,0 +1,152 @@
+theory IsaSAT_Print_LLVM
+  imports IsaSAT_Literals_LLVM
+begin
+
+definition print_propa :: \<open>64 word \<Rightarrow> unit\<close> where
+  \<open>print_propa _ = ()\<close>
+
+definition print_confl :: \<open>64 word \<Rightarrow> unit\<close> where
+  \<open>print_confl _ = ()\<close>
+
+definition print_dec :: \<open>64 word \<Rightarrow> unit\<close> where
+  \<open>print_dec _ = ()\<close>
+
+definition print_res :: \<open>64 word \<Rightarrow> unit\<close> where
+  \<open>print_res _ = ()\<close>
+
+definition print_lres :: \<open>64 word \<Rightarrow> unit\<close> where
+  \<open>print_lres _ = ()\<close>
+
+definition print_uset :: \<open>64 word \<Rightarrow> unit\<close> where
+  \<open>print_uset _ = ()\<close>
+
+definition print_gcs :: \<open>64 word \<Rightarrow> unit\<close> where
+  \<open>print_gcs _ = ()\<close>
+
+definition print_binary_unit :: \<open>64 word \<Rightarrow> unit\<close> where
+  \<open>print_binary_unit _ = ()\<close>
+
+definition print_binary_red_removed :: \<open>64 word \<Rightarrow> unit\<close> where
+  \<open>print_binary_red_removed _ = ()\<close>
+
+definition print_purelit_elim :: \<open>64 word \<Rightarrow> unit\<close> where
+  \<open>print_purelit_elim _ = ()\<close>
+
+definition print_purelit_rounds :: \<open>64 word \<Rightarrow> unit\<close> where
+  \<open>print_purelit_rounds _ = ()\<close>
+
+definition print_lbds :: \<open>64 word \<Rightarrow> unit\<close> where
+  \<open>print_lbds _ = ()\<close>
+
+definition print_forward_rounds :: \<open>64 word \<Rightarrow> unit\<close> where
+  \<open>print_forward_rounds _ = ()\<close>
+
+definition print_forward_subsumed :: \<open>64 word \<Rightarrow> 64 word \<Rightarrow> unit\<close> where
+  \<open>print_forward_subsumed _ _ = ()\<close>
+
+definition print_forward_tried :: \<open>64 word \<Rightarrow> unit\<close> where
+  \<open>print_forward_tried _ = ()\<close>
+
+definition print_forward_strengthened :: \<open>64 word \<Rightarrow> 64 word \<Rightarrow> unit\<close> where
+  \<open>print_forward_strengthened _ _ = ()\<close>
+
+sepref_def print_propa_impl
+  is \<open>RETURN o print_propa\<close>
+  :: \<open>word_assn\<^sup>k \<rightarrow>\<^sub>a unit_assn\<close>
+  unfolding print_propa_def
+  by sepref
+
+sepref_def print_confl_impl
+  is \<open>RETURN o print_confl\<close>
+  :: \<open>word_assn\<^sup>k \<rightarrow>\<^sub>a unit_assn\<close>
+  unfolding print_confl_def
+  by sepref
+
+sepref_def print_dec_impl
+  is \<open>RETURN o print_dec\<close>
+  :: \<open>word_assn\<^sup>k \<rightarrow>\<^sub>a unit_assn\<close>
+  unfolding print_dec_def
+  by sepref
+
+sepref_def print_res_impl
+  is \<open>RETURN o print_res\<close>
+  :: \<open>word_assn\<^sup>k \<rightarrow>\<^sub>a unit_assn\<close>
+  unfolding print_res_def
+  by sepref
+
+sepref_def print_lres_impl
+  is \<open>RETURN o print_lres\<close>
+  :: \<open>word_assn\<^sup>k \<rightarrow>\<^sub>a unit_assn\<close>
+  unfolding print_lres_def
+  by sepref
+
+sepref_def print_uset_impl
+  is \<open>RETURN o print_uset\<close>
+  :: \<open>word_assn\<^sup>k \<rightarrow>\<^sub>a unit_assn\<close>
+  unfolding print_uset_def
+  by sepref
+
+definition print_irred_clss :: \<open>64 word \<Rightarrow> unit\<close> where
+  \<open>print_irred_clss _ = ()\<close>
+
+sepref_def print_gc_impl
+  is \<open>RETURN o print_gcs\<close>
+  :: \<open>word_assn\<^sup>k \<rightarrow>\<^sub>a unit_assn\<close>
+  unfolding print_gcs_def
+  by sepref
+
+sepref_def print_irred_clss_impl
+  is \<open>RETURN o print_irred_clss\<close>
+  :: \<open>word_assn\<^sup>k \<rightarrow>\<^sub>a unit_assn\<close>
+  unfolding print_irred_clss_def
+  by sepref
+
+sepref_def print_binary_unit_impl
+  is \<open>RETURN o print_binary_unit\<close>
+  :: \<open>word_assn\<^sup>k \<rightarrow>\<^sub>a unit_assn\<close>
+  unfolding print_binary_unit_def
+  by sepref
+
+sepref_def print_purelit_rounds_impl
+  is \<open>RETURN o print_purelit_rounds\<close>
+  :: \<open>word_assn\<^sup>k \<rightarrow>\<^sub>a unit_assn\<close>
+  unfolding print_purelit_rounds_def
+  by sepref
+
+sepref_def print_purelit_elim_impl
+  is \<open>RETURN o print_purelit_elim\<close>
+  :: \<open>word_assn\<^sup>k \<rightarrow>\<^sub>a unit_assn\<close>
+  unfolding print_purelit_elim_def
+  by sepref
+
+sepref_def print_binary_red_removed_impl
+  is \<open>RETURN o print_binary_red_removed\<close>
+  :: \<open>word_assn\<^sup>k \<rightarrow>\<^sub>a unit_assn\<close>
+  unfolding print_binary_red_removed_def
+  by sepref
+
+sepref_def print_forward_rounds_impl
+  is \<open>RETURN o print_forward_rounds\<close>
+  :: \<open>word_assn\<^sup>k \<rightarrow>\<^sub>a unit_assn\<close>
+  unfolding print_forward_rounds_def
+  by sepref
+
+sepref_def print_forward_subsumed_impl
+  is \<open>uncurry (RETURN oo print_forward_subsumed)\<close>
+  :: \<open>word_assn\<^sup>k *\<^sub>a word_assn\<^sup>k \<rightarrow>\<^sub>a unit_assn\<close>
+  unfolding print_forward_subsumed_def
+  by sepref
+
+sepref_def print_forward_tried_impl
+  is \<open>RETURN o print_forward_tried\<close>
+  :: \<open>word_assn\<^sup>k \<rightarrow>\<^sub>a unit_assn\<close>
+  unfolding print_forward_tried_def
+  by sepref
+
+sepref_def print_forward_strengthened_impl
+  is \<open>uncurry (RETURN oo print_forward_strengthened)\<close>
+  :: \<open>word_assn\<^sup>k *\<^sub>a word_assn\<^sup>k \<rightarrow>\<^sub>a unit_assn\<close>
+  unfolding print_forward_strengthened_def
+  by sepref
+
+end
